More precise neededness analysis of 64-bit integer operations
Especially the conversions between 32 and 64-bit integers, but also:
- x86: the `leal` operation
- aarch64: various combined operations (extend and shift, extend and shift and add, etc).

x86/NeedOp.v
@@ -25,7 +25,7 @@ Definition needs_of_condition (cond: condition): list nval :=
   | _ => nil
   end.
 
-Definition needs_of_addressing_32 (addr: addressing) (nv: nval): list nval :=
+Definition needs_of_addressing (addr: addressing) (nv: nval): list nval :=
   match addr with
   | Aindexed n => op1 (modarith nv)
   | Aindexed2 n => op2 (modarith nv)
@@ -36,21 +36,6 @@ Definition needs_of_addressing_32 (addr: addressing) (nv: nval): list nval :=
   | Abasedscaled sc s ofs => op1 (modarith (modarith nv))
   | Ainstack ofs => nil
   end.
-
-Definition needs_of_addressing_64 (addr: addressing) (nv: nval): list nval :=
-  match addr with
-  | Aindexed n => op1 (default nv)
-  | Aindexed2 n => op2 (default nv)
-  | Ascaled sc ofs => op1 (default nv)
-  | Aindexed2scaled sc ofs => op2 (default nv)
-  | Aglobal s ofs => nil
-  | Abased s ofs => op1 (default nv)
-  | Abasedscaled sc s ofs => op1 (default nv)
-  | Ainstack ofs => nil
-  end.
-
-Definition needs_of_addressing (addr: addressing) (nv: nval): list nval :=
-  if Archi.ptr64 then needs_of_addressing_64 addr nv else needs_of_addressing_32 addr nv.
 
 Definition needs_of_operation (op: operation) (nv: nval): list nval :=
   match op with
@@ -85,11 +70,12 @@ Definition needs_of_operation (op: operation) (nv: nval): list nval :=
   | Oshruimm n => op1 (shruimm nv n)
   | Ororimm n => op1 (ror nv n)
   | Oshldimm n => op1 (default nv)
-  | Olea addr => needs_of_addressing_32 addr nv
-  | Omakelong => op2 (default nv)
-  | Olowlong | Ohighlong => op1 (default nv)
-  | Ocast32signed => op1 (default nv)
-  | Ocast32unsigned => op1 (default nv)
+  | Olea addr => needs_of_addressing addr nv
+  | Omakelong => makelong_hi nv :: makelong_lo nv :: nil
+  | Olowlong => op1 (loword nv)
+  | Ohighlong => op1 (hiword nv)
+  | Ocast32signed => op1 (longofint nv)
+  | Ocast32unsigned => op1 (longofintu nv)
   | Onegl => op1 (modarith nv)
   | Oaddlimm _ => op1 (modarith nv)
   | Osubl => op2 (default nv)
@@ -111,7 +97,7 @@ Definition needs_of_operation (op: operation) (nv: nval): list nval :=
   | Oshrlu => op2 (default nv)
   | Oshrluimm n => op1 (shrluimm nv n)
   | Ororlimm n => op1 (rorl nv n)
-  | Oleal addr => needs_of_addressing_64 addr nv
+  | Oleal addr => needs_of_addressing addr nv
   | Onegf | Oabsf => op1 (default nv)
   | Oaddf | Osubf | Omulf | Odivf | Omaxf | Ominf => op2 (default nv)
   | Onegfs | Oabsfs => op1 (default nv)
@@ -173,28 +159,34 @@ Qed.
 Lemma needs_of_addressing_32_sound:
   forall sp addr args v nv args',
   eval_addressing32 ge (Vptr sp Ptrofs.zero) addr args = Some v ->
-  vagree_list args args' (needs_of_addressing_32 addr nv) ->
+  vagree_list args args' (needs_of_addressing addr nv) ->
   exists v',
      eval_addressing32 ge (Vptr sp Ptrofs.zero) addr args' = Some v'
   /\ vagree v v' nv.
 Proof.
-  unfold needs_of_addressing_32; intros.
+  unfold needs_of_addressing; intros.
   destruct addr; simpl in *; FuncInv; InvAgree; TrivialExists;
   auto using add_sound, mul_sound with na.
-  apply add_sound; auto with na. apply add_sound; rewrite modarith_idem; auto.
-  apply add_sound; auto. apply add_sound; rewrite modarith_idem; auto with na.
+- apply add_sound; auto with na. apply add_sound; rewrite modarith_idem; auto.
+- apply add_sound; auto. apply add_sound; rewrite modarith_idem; auto with na.
   apply mul_sound; rewrite modarith_idem; auto with na.
 Qed.
 
-(*
 Lemma needs_of_addressing_64_sound:
   forall sp addr args v nv args',
   eval_addressing64 ge (Vptr sp Ptrofs.zero) addr args = Some v ->
-  vagree_list args args' (needs_of_addressing_64 addr nv) ->
+  vagree_list args args' (needs_of_addressing addr nv) ->
   exists v',
      eval_addressing64 ge (Vptr sp Ptrofs.zero) addr args' = Some v'
   /\ vagree v v' nv.
-*)
+Proof.
+  unfold needs_of_addressing; intros.
+  destruct addr; simpl in *; FuncInv; InvAgree; TrivialExists;
+  auto using addl_sound, mull_sound with na.
+- apply addl_sound; auto with na. apply addl_sound; rewrite modarith_idem; auto.
+- apply addl_sound; auto with na. apply addl_sound; auto with na.
+  apply mull_sound; rewrite ! modarith_idem; auto with na.
+Qed.
 
 Lemma needs_of_operation_sound:
   forall op args v nv args',
@@ -226,6 +218,11 @@ Proof.
 - apply shruimm_sound; auto.
 - apply ror_sound; auto.
 - eapply needs_of_addressing_32_sound; eauto.
+- apply makelong_sound; auto.
+- apply loword_sound; auto.
+- apply hiword_sound; auto.
+- apply longofint_sound; auto.
+- apply longofintu_sound; auto.
 - apply negl_sound; auto.
 - apply addl_sound; auto with na.
 - apply mull_sound; auto.
@@ -241,10 +238,7 @@ Proof.
 - apply shrlimm_sound; auto.
 - apply shrluimm_sound; auto.
 - apply rorl_sound; auto.
-- change (eval_addressing64 ge (Vptr sp Ptrofs.zero) a args')
-    with (eval_operation ge (Vptr sp Ptrofs.zero) (Oleal a) args' m').
-  eapply default_needs_of_operation_sound; eauto.
-  destruct a; simpl in H0; auto.
+- eapply needs_of_addressing_64_sound; eauto.
 - destruct (eval_condition cond args m) as [b|] eqn:EC; simpl in H2.
   erewrite needs_of_condition_sound by eauto.
   subst v; simpl. auto with na.
